@prefix : <https://parallax.nmsu.edu/> .
@prefix bfo: <http://purl.obolibrary.org/obo/BFO> .
@prefix cco: <https://www.commoncoreontologies.org/> .
@prefix owl: <http://www.w3.org/2002/07/owl#> .
@prefix rdf: <http://www.w3.org/1999/02/22-rdf-syntax-ns#> .
@prefix xml: <http://www.w3.org/XML/1998/namespace> .
@prefix xsd: <http://www.w3.org/2001/XMLSchema#> .
@prefix envo: <http://purl.obolibrary.org/obo/ENVO> .
@prefix rdfs: <http://www.w3.org/2000/01/rdf-schema#> .
@prefix skos: <http://www.w3.org/2004/02/skos/core#> .
@prefix sosa: <http://www.w3.org/ns/sosa/> .
@prefix schema: <http://schema.org/> .
@prefix parallax: <https://parallax.nmsu.edu/> .
@base <https://parallax.nmsu.edu/> .

<https://parallax.nmsu.edu/ns/> rdf:type owl:Ontology ;
                                 owl:imports <http://purl.obolibrary.org/obo/bfo/2020/bfo-core.owl> .

#################################################################
#    Annotation properties
#################################################################

###  http://schema.org/domainIncludes
schema:domainIncludes rdf:type owl:AnnotationProperty .


###  http://schema.org/rangeIncludes
schema:rangeIncludes rdf:type owl:AnnotationProperty .


###  https://www.commoncoreontologies.org/ont00001754
cco:ont00001754 rdf:type owl:AnnotationProperty .


###  https://www.commoncoreontologies.org/ont00001760
cco:ont00001760 rdf:type owl:AnnotationProperty .


#################################################################
#    Object Properties
#################################################################

###  http://www.w3.org/ns/sosa/hasFeatureOfInterest
sosa:hasFeatureOfInterest rdf:type owl:ObjectProperty ;
                          owl:inverseOf sosa:isFeatureOfInterestOf ;
                          schema:domainIncludes sosa:Actuation ,
                                                sosa:Observation ,
                                                sosa:Sampling ;
                          schema:rangeIncludes sosa:FeatureOfInterest ,
                                               sosa:Sample ;
                          rdfs:comment "A relation between an Observation and the entity whose quality was observed, or between an Actuation and the entity whose property was modified, or between an act of Sampling and the entity that was sampled."@en ;
                          rdfs:isDefinedBy sosa: ;
                          rdfs:label "has feature of interest"@en ;
                          skos:definition "A relation between an Observation and the entity whose quality was observed, or between an Actuation and the entity whose property was modified, or between an act of Sampling and the entity that was sampled."@en ;
                          skos:example "For example, in an Observation of the weight of a person, the FeatureOfInterest is the person and the property is its weight."@en .


###  http://www.w3.org/ns/sosa/isFeatureOfInterestOf
sosa:isFeatureOfInterestOf rdf:type owl:ObjectProperty .


#################################################################
#    Data properties
#################################################################

###  http://www.w3.org/ns/sosa/resultTime
sosa:resultTime rdf:type owl:DatatypeProperty ;
                rdfs:range xsd:dateTime ;
                schema:domainIncludes sosa:Actuation ,
                                      sosa:Observation ,
                                      sosa:Sampling ;
                rdfs:comment "The result time is the instant of time when the Observation, Actuation or Sampling activity was completed."@en ;
                rdfs:isDefinedBy sosa: ;
                rdfs:label "result time"@en ;
                skos:definition "The result time is the instant of time when the Observation, Actuation or Sampling activity was completed."@en .


###  https://www.commoncoreontologies.org/ont00001764
cco:ont00001764 rdf:type owl:DatatypeProperty ;
                rdfs:range xsd:decimal ;
                rdfs:label "has longitude value"@en ;
                skos:definition "A Data Property that has as its range the longitude value from some Geospatial Location coordinates set expressed in decimal degrees."@en ;
                cco:ont00001760 "https://www.commoncoreontologies.org/GeospatialOntology"^^xsd:anyURI .


###  https://www.commoncoreontologies.org/ont00001766
cco:ont00001766 rdf:type owl:DatatypeProperty ;
                rdfs:range xsd:decimal ;
                rdfs:label "has latitude value"@en ;
                skos:definition "A Data Property that has as its range the latitude value from some Geospatial Location coordinates set expressed in decimal degrees."@en ;
                cco:ont00001760 "https://www.commoncoreontologies.org/GeospatialOntology"^^xsd:anyURI .


#################################################################
#    Classes
#################################################################

###  http://purl.obolibrary.org/obo/ENVO_00000463
envo:_00000463 rdf:type owl:Class ;
               rdfs:subClassOf bfo:_0000029 ;
               rdfs:comment "Copied temporarily from ENVO. Replace with MIREOT import." ;
               rdfs:label "harbour" .


###  http://purl.obolibrary.org/obo/ENVO_01000605
envo:_01000605 rdf:type owl:Class ;
               rdfs:subClassOf bfo:_0000030 ;
               rdfs:comment "Copied temporarily from ENVO. Replace with MIREOT import." ;
               rdfs:label "car" .


###  http://purl.obolibrary.org/obo/ENVO_01000608
envo:_01000608 rdf:type owl:Class ;
               rdfs:subClassOf bfo:_0000030 ;
               rdfs:comment "Copied temporarily from ENVO. Replace with MIREOT import." ;
               rdfs:label "boat" .


###  http://purl.obolibrary.org/obo/ENVO_03501349
envo:_03501349 rdf:type owl:Class ;
               rdfs:subClassOf bfo:_0000030 ;
               rdfs:comment "Copied temporarily from ENVO. Replace with MIREOT import." ;
               rdfs:label "airplane" .


###  http://www.w3.org/ns/sosa/Observation
sosa:Observation rdf:type owl:Class ;
                 rdfs:subClassOf bfo:_0000015 ;
                 rdfs:comment "Act of carrying out an (Observation) Procedure to estimate or calculate a value of a property of a FeatureOfInterest. Links to a Sensor to describe what made the Observation and how; links to an ObservableProperty to describe what the result is an estimate of, and to a FeatureOfInterest to detail what that property was associated with."@en ;
                 rdfs:isDefinedBy sosa: ;
                 rdfs:label "Observation"@en ;
                 skos:definition "Act of carrying out an (Observation) Procedure to estimate or calculate a value of a property of a FeatureOfInterest. Links to a Sensor to describe what made the Observation and how; links to an ObservableProperty to describe what the result is an estimate of, and to a FeatureOfInterest to detail what that property was associated with."@en ;
                 skos:example "The activity of estimating the intensity of an Earthquake using the Mercalli intensity scale is an Observation as is measuring the moment magnitude, i.e., the energy released by said earthquake."@en .


###  https://parallax.nmsu.edu/ns/BoatObservation
:BoatObservation rdf:type owl:Class ;
                 rdfs:subClassOf sosa:Observation ,
                                 [ rdf:type owl:Restriction ;
                                   owl:onProperty sosa:hasFeatureOfInterest ;
                                   owl:someValuesFrom envo:_01000608
                                 ] .


###  https://www.commoncoreontologies.org/ont00000005
cco:ont00000005 rdf:type owl:Class ;
                rdfs:subClassOf bfo:_0000015 ;
                rdfs:label "Act"@en ;
                skos:definition "A Process in which at least one Agent plays a causative role."@en ;
                cco:ont00001760 "https://www.commoncoreontologies.org/EventOntology"^^xsd:anyURI .


###  https://www.commoncoreontologies.org/ont00000065
cco:ont00000065 rdf:type owl:Class ;
                rdfs:subClassOf cco:ont00000357 ;
                rdfs:label "Act of Location Change"@en ;
                skos:definition "An Act of Motion in which the location of some Object is changed by some Agent."@en ;
                cco:ont00001760 "https://www.commoncoreontologies.org/EventOntology"^^xsd:anyURI .


###  https://www.commoncoreontologies.org/ont00000228
cco:ont00000228 rdf:type owl:Class ;
                rdfs:subClassOf cco:ont00000005 ;
                rdfs:label "Planned Act"@en ;
                skos:altLabel "Intentional Act"@en ;
                skos:definition "An Act in which at least one Agent plays a causative role and which is prescribed by some Directive Information Content Entity held by at least one of the Agents."@en ;
                cco:ont00001760 "https://www.commoncoreontologies.org/EventOntology"^^xsd:anyURI .


###  https://www.commoncoreontologies.org/ont00000357
cco:ont00000357 rdf:type owl:Class ;
                rdfs:subClassOf cco:ont00000228 ;
                rdfs:label "Act of Motion"@en ;
                skos:definition "A Planned Act by which an Agent causes the position or location of some Object to change."@en ;
                cco:ont00001754 "http://www.merriam-webster.com/dictionary/motion" ;
                cco:ont00001760 "https://www.commoncoreontologies.org/EventOntology"^^xsd:anyURI .


###  https://www.commoncoreontologies.org/ont00000890
cco:ont00000890 rdf:type owl:Class ;
                rdfs:subClassOf cco:ont00000065 ;
                rdfs:label "Act of Travel"@en ;
                skos:definition "An Act of Location Change wherein one or more Persons move between relatively distant geographical locations for any purpose and any duration, with or without any means of transport."@en ;
                cco:ont00001754 "https://en.wikipedia.org/w/index.php?title=Travel&oldid=1037229469"^^xsd:anyURI ;
                cco:ont00001760 "https://www.commoncoreontologies.org/EventOntology"^^xsd:anyURI .


###  Generated by the OWL API (version 4.5.29.2024-05-13T12:11:03Z) https://github.com/owlcs/owlapi
